Object_Model.thy
@@ -112,23 +112,175 @@ definition "attrs1 \<equiv> fmap_of_list [
     (STR ''cost'', Real[?])]),
   (Task, fmap_of_list [
     (STR ''description'', String[1])])]"
-
+(*
+lemma subclass1_code [code_pred_intro]:
+  "(cls :: classes1) \<le> cls"
+  "subclass1 cls cls2 \<Longrightarrow>
+   cls \<le> cls2"
+  by (simp_all add: less_classes1_def less_eq_classes1_def)
+*)
 lemma find_attribute_code [code_pred_intro]:
-  "fmlookup attrs cls2 = Some cls_attrs \<Longrightarrow>
+  "fmlookup attrs cls = Some cls_attrs \<Longrightarrow>
    fmlookup cls_attrs name = Some \<tau> \<Longrightarrow>
-   cls = cls2 \<Longrightarrow>
-   find_attribute attrs cls name cls2 \<tau>"
-  "fmlookup attrs cls2 = Some cls_attrs \<Longrightarrow>
+   find_attribute attrs cls name cls \<tau>"
+  "subclass1 cls cls2 \<Longrightarrow>
+   fmlookup attrs cls2 = Some cls_attrs \<Longrightarrow>
    fmlookup cls_attrs name = Some \<tau> \<Longrightarrow>
-   subclass1 cls cls2 \<Longrightarrow>
    find_attribute attrs cls name cls2 \<tau>"
-  by (simp_all add: find_attribute.intros dual_order.strict_implies_order less_classes1_def)
+  by (simp_all add: find_attribute.intros less_classes1_def less_eq_classes1_def)
 
+(*
+datatype ty = A | B | C
+
+inductive lty where
+  "lty A C"
+| "lty B C"
+
+instantiation ty :: order
+begin
+
+definition "(<) \<equiv> lty"
+definition "x \<le> y \<equiv> x = y \<or> lty x y"
+
+instance
+  apply intro_classes
+  using less_eq_ty_def less_ty_def lty.simps by auto
+
+end
+
+inductive pred1 where
+  "x \<le> y \<Longrightarrow>
+   pred1 x y"
+
+lemma pred1_ty_code [code_pred_intro]:
+  "x = y \<Longrightarrow>
+   pred1 x y"
+  "lty x y \<Longrightarrow>
+   pred1 x y"
+  by (simp_all add: less_eq_ty_def pred1.intros r_into_rtranclp)
+
+code_pred [show_modes] pred1
+  using less_eq_ty_def pred1.simps by blast
+
+values "{x. pred1 A x}"
+
+
+inductive pred2 where
+  "pred1 x y \<Longrightarrow>
+   pred2 x y"
+
+(*
+lemma pred2_ty_code [code_pred_intro]:
+  "pred1 x y \<Longrightarrow>
+   pred2 x y"
+  by (simp_all add: pred1_ty_code pred2.intros)
+
+code_pred [show_modes] pred2
+  using pred2.cases by blast
+*)
+lemma pred2_ty_code [code_pred_intro]:
+  "x = y \<Longrightarrow>
+   pred2 x y"
+  "lty x y \<Longrightarrow>
+   pred2 x y"
+  by (simp_all add: pred1_ty_code pred2.intros)
+
+code_pred [show_modes] pred2
+  using less_eq_ty_def pred1.cases pred2.simps by blast
+
+values "{x. pred2 A x}"
+
+
+
+
+
+datatype ty = A | B | C | D
+
+inductive lty where
+  "lty A C"
+| "lty B C"
+| "lty C D"
+
+inductive_cases lty_x_A [elim!]: "lty x A"
+inductive_cases lty_x_B [elim!]: "lty x B"
+inductive_cases lty_x_C [elim!]: "lty x C"
+inductive_cases lty_x_D [elim!]: "lty x D"
+
+code_pred [show_modes] lty .
+
+instantiation ty :: order
+begin
+
+definition "(<) \<equiv> lty\<^sup>+\<^sup>+"
+definition "(\<le>) \<equiv> lty\<^sup>*\<^sup>*"
+
+lemma ty_less_le_not_le:
+  "x < y \<longleftrightarrow> x \<le> y \<and> \<not> (y \<le> x)"
+  for x y :: ty
+  unfolding less_ty_def less_eq_ty_def
+  apply auto
+  apply (metis Nitpick.rtranclp_unfold lty.cases lty_x_A lty_x_B lty_x_C tranclp.cases tranclpD)
+  by (metis rtranclpD)
+
+instance
+  apply intro_classes
+  apply (simp add: ty_less_le_not_le)
+  apply (simp add: less_eq_ty_def)
+  apply (metis less_eq_ty_def rtranclp_trans)
+  by (metis (mono_tags, lifting) less_eq_ty_def less_ty_def rtranclpD ty_less_le_not_le)
+
+end
+
+inductive pred1 where
+  "x \<le> y \<Longrightarrow>
+   pred1 x y"
+
+inductive pred2 where
+  "pred1 x y \<Longrightarrow>
+   pred2 x y"
+
+lemma pred1_ty_code [code_pred_intro]:
+  "x = y \<Longrightarrow>
+   pred1 x y"
+  "lty x y \<Longrightarrow>
+   pred1 x y"
+  by (simp_all add: less_eq_ty_def pred1.intros r_into_rtranclp)
+
+code_pred [show_modes] pred1
+  apply (erule pred1.cases)
+*)
 code_pred [show_modes] find_attribute
-  by (metis find_attribute.cases le_neq_trans less_classes1_def)
+  by (metis find_attribute.cases less_classes1_def less_eq_classes1_def)
 
 values "{(c, t). find_attribute attrs1 Employee (STR ''name'') c t}"
 values "{(c, t). find_attribute attrs1 Employee (STR ''position'') c t}"
+(*
+inductive elems where
+  "x |\<in>| xs \<Longrightarrow>
+   elems xs x"
+
+primrec elems_fun where
+  "elems_fun "
+
+term "set_of_pred"
+term subclass1_i_o
+value "set_of_pred (subclass1_i_o Employee)"
+
+code_pred [show_modes] elems .
+
+values "{x. elems {|1::nat,2,3|} x}"
+
+lemma find_assoc1_code [code_pred_intro]:
+  "find_assoc1 assocs (fmdom assocs)"
+*)
+
+inductive find_assoc where
+  "a |\<in>| fmdom assocs \<Longrightarrow>
+   fmlookup assocs a = Some assoc \<Longrightarrow>
+   fmlookup assoc name = Some end \<Longrightarrow>
+   find_assoc assocs cls name end"
+
+code_pred [show_modes] find_assoc .
 
 definition assocs1 :: "classes1 assocs" where
   "assocs1 \<equiv> fmap_of_list [
@@ -187,16 +339,15 @@ definition sorted_list_of_assocs :: "'a assocs \<Rightarrow> 'a binary_assoc lis
     map (\<lambda>(assoc, roles).
       map (\<lambda>(from, ends).
         map (\<lambda>end. (assoc, end)) ends) roles)
-    (sorted_list_of_fmap (fmmap
-      (\<lambda>xm. sorted_list_of_fmap (fmmap_keys
-        (\<lambda>x v. map (\<lambda>y. (x, v, y)) (sorted_list_of_fmap (fmdrop x xm))) xm))
-      assocs))))"
+      (sorted_list_of_fmap (fmmap (\<lambda>xm.
+        (sorted_list_of_fmap (fmmap_keys (\<lambda>x v. map (\<lambda>y. (x, v, y))
+          (sorted_list_of_fmap (fmdrop x xm))) xm))) assocs))))"
 
 definition "roles xs \<equiv> map (\<lambda>assoc. (assoc_end_class (from_assoc_end assoc), assoc)) xs"
 
 value "roles (sorted_list_of_assocs assocs1)"
 value "sorted_list_of_assocs assocs1"
-
+(*
 definition "sorted_list_of_assocs assocs \<equiv>
    (fold (\<lambda>(a, r) y. y @ [fold (\<lambda>(x, y) z. z @ [(a, y)]) r []])
     (sorted_list_of_fmap (fmmap (\<lambda>xm.
@@ -210,7 +361,7 @@ definition "sorted_list_of_assocs assocs \<equiv>
       map (\<lambda>x. map (\<lambda>y. (x, y)) (sorted_list_of_fmap (fmdrop x xm)))
           (sorted_list_of_fset (fmdom xm)))
       assocs)) [])"
-
+*)
 
 value "let x = fmap_of_list [
     (STR ''manages'', (Project, 0::nat, 2::nat)),
@@ -220,11 +371,11 @@ value "let x = fmap_of_list [
 term "fmdrop"
 
 value "fmmap sorted_list_of_fmap assocs1"
-
+(*
 definition "sorted_list_of_assocs assocs \<equiv>
    (fold (\<lambda>(a, r) y. y @ [fold (\<lambda>x z. z @ [(a, x)]) r []])
     (sorted_list_of_fmap (fmmap sorted_list_of_fmap assocs)) [])"
-
+*)
 value "assocs1"
 
 term fmmap
@@ -232,9 +383,9 @@ term "(fmmap_keys (\<lambda>k v. (k, sorted_list_of_fmap v)) assocs1)"
 term "(sorted_list_of_fmap (fmmap_keys (\<lambda>k v. (sorted_list_of_fmap v)) assocs1))"
 
 value "[[1::nat,2],[3,4,5],[6,7]]"
-
+(*
 value "fold (\<lambda>x y. product_lists [y,y]) [[1::nat,2],[3,4,5],[6,7]] ([] :: nat list)"
-
+*)
 value "product [[1::nat,2],[3,4,5],[6,7]]"
 term "product"
 value "subseqs [1::nat, 2, 3]"
@@ -247,10 +398,11 @@ primrec n_lists :: "nat \<Rightarrow> 'a list \<Rightarrow> 'a list list" where
 "n_lists 0 xs = [[]]" |
 "n_lists (Suc n) xs = concat (map (\<lambda>ys. map (\<lambda>y. y # ys) xs) (n_lists n xs))"
 *)
+(*
 primrec n_lists :: "'a list \<Rightarrow> ('a \<times> 'a) list" where
 "n_lists 0 xs = [[]]" |
 "n_lists (Suc n) xs = concat (map (\<lambda>ys. map (\<lambda>y. y # ys) xs) (n_lists n xs))"
-
+*)
 term filter
 value "n_lists 2 [1::nat,2,3]"
 value "shuffle [1::nat,2] [3,4]"
@@ -278,31 +430,32 @@ term "ffold (\<lambda>(a, r, e) y. ffold (\<lambda>x z. finsert (a, r, x) z) fem
 
 term "fset_of_fmap (fmmap_keys (\<lambda>k v. (k, fset_of_fmap v)) assocs1)"
 
-
-
-
-
 inductive find_association where
-  "(*cls \<le> cls2 \<Longrightarrow>*)
-   (*find_assocs assocs cls name = a1 \<Longrightarrow>*)
-   fset_of_fmap assocs = a1 \<Longrightarrow>
-   (*assoc_refer_class (fmdrop name ends) cls \<Longrightarrow>
-   fmlookup ends name = Some end \<Longrightarrow>
-   assocs = (fmupd assoc ends assocs2) \<Longrightarrow>*)
-   find_association assocs cls name a1"
+  "cls \<le> cls2 \<Longrightarrow>
+   find_assoc_end assocs cls2 name = Some end \<Longrightarrow>
+   find_association assocs cls name cls2 end"
 
-code_pred [show_modes] find_association .
+lemma find_association_code [code_pred_intro]:
+  "find_assoc_end assocs cls name = Some end \<Longrightarrow>
+   find_association assocs cls name cls end"
+  "subclass1 cls cls2 \<Longrightarrow>
+   find_assoc_end assocs cls2 name = Some end \<Longrightarrow>
+   find_association assocs cls name cls2 end"
+  by (simp_all add: find_association.intros less_eq_classes1_def less_classes1_def)
 
-values "{x. find_association assocs1 Project ''manager'' x}"
-values "{x. find_association assocs1 Project ''manager1'' x}"
+code_pred [show_modes] find_association
+  by (metis find_association.cases less_classes1_def less_eq_classes1_def)
 
-value "find_assocs assocs1 Project ''manager''"
-value "find_assocs assocs1 Employee ''tasks''"
-value "find_assoc_end assocs1 Project ''manager''"
-value "find_assoc_end assocs1 Employee ''tasks''"
+values "{(c, e). find_association assocs1 Project STR ''manager'' c e}"
+values "{(c, e). find_association assocs1 Project STR ''manager1'' c e}"
 
-value "find_assocs assocs1 Project ''manager1''"
-value "find_assoc_end assocs1 Project ''manager1''"
+value "find_assocs assocs1 Project STR ''manager''"
+value "find_assocs assocs1 Employee STR ''tasks''"
+value "find_assoc_end assocs1 Project STR ''manager''"
+value "find_assoc_end assocs1 Employee STR ''tasks''"
+
+value "find_assocs assocs1 Project STR ''manager1''"
+value "find_assoc_end assocs1 Project STR ''manager1''"
 
 
 
@@ -314,14 +467,14 @@ definition "model1 \<equiv> (attrs1, assocs1)"
 
 subsection \<open>Positive Cases\<close>
 
-value "find_assocs assocs1 Project ''manager''"
-value "find_assocs assocs1 Employee ''tasks''"
-value "find_assoc_end assocs1 Project ''manager''"
-value "find_assoc_end assocs1 Employee ''tasks''"
+value "find_assocs assocs1 Project STR ''manager''"
+value "find_assocs assocs1 Employee STR ''tasks''"
+value "find_assoc_end assocs1 Project STR ''manager''"
+value "find_assoc_end assocs1 Employee STR ''tasks''"
 
 subsection \<open>Negative Cases\<close>
 
-value "find_assocs assocs1 Project ''manager1''"
-value "find_assoc_end assocs1 Project ''manager1''"
+value "find_assocs assocs1 Project STR ''manager1''"
+value "find_assoc_end assocs1 Project STR ''manager1''"
 
 end
